worked on the definition of the semantic and some proofs

src/equiv_rel.v
@@ -29,10 +29,10 @@ Definition opt_rel {A : Type} (R : A -> A -> Prop) (e1 e2 : option A) : Prop :=
     end.
 
 Definition deq_rel (d1 d2 : deq) :=
-    forall prog ctxt, opt_rel context_rel (eval_deq arch prog ctxt d1) (eval_deq arch prog ctxt d2).
+    forall prog type_ctxt ctxt, opt_rel context_rel (eval_deq arch prog type_ctxt ctxt d1) (eval_deq arch prog type_ctxt ctxt d2).
 
 Definition deqs_rel (dl1 dl2 : list_deq) :=
-    forall prog ctxt, opt_rel context_rel (eval_deq_list arch prog ctxt dl1) (eval_deq_list arch prog ctxt dl2).
+    forall prog type_ctxt ctxt, opt_rel context_rel (eval_deq_list arch prog type_ctxt ctxt dl1) (eval_deq_list arch prog type_ctxt ctxt dl2).
 
 (* Properties on relations *)
 
@@ -148,8 +148,8 @@ Proof. unfold deq_rel; intros; symmetry; auto. Qed.
 
 Lemma deq_rel_trans: forall d1 d2 d3, deq_rel d1 d2 -> deq_rel d2 d3 -> deq_rel d1 d3.
 Proof.
-    unfold deq_rel; move=> d1 d2 d3 Eq1 Eq2 prog ctxt.
-    transitivity (eval_deq arch prog ctxt d2); auto.
+    unfold deq_rel; move=> d1 d2 d3 Eq1 Eq2 prog type_ctxt ctxt.
+    transitivity (eval_deq arch prog type_ctxt ctxt d2); auto.
 Qed.
 
 #[global]
@@ -170,8 +170,8 @@ Proof. unfold deqs_rel; intros; symmetry; auto. Qed.
 
 Lemma deqs_rel_trans: forall d1 d2 d3, deqs_rel d1 d2 -> deqs_rel d2 d3 -> deqs_rel d1 d3.
 Proof.
-    unfold deqs_rel; move=> d1 d2 d3 Eq1 Eq2 prog ctxt.
-    transitivity (eval_deq_list arch prog ctxt d2); auto.
+    unfold deqs_rel; move=> d1 d2 d3 Eq1 Eq2 prog type_ctxt ctxt.
+    transitivity (eval_deq_list arch prog type_ctxt ctxt d2); auto.
 Qed.
 
 #[global]
@@ -238,96 +238,7 @@ Proof.
     all: rewrite Hypo; trivial.
 Qed.
 
-
-Lemma context_srel_bind_compl:
-    forall var val ctxt,
-        match bind ctxt var val with
-        | Some ctxt' => context_srel (Complement ident (var_freevars var)) ctxt ctxt'
-        | None => True
-        end.
-Proof.
-    move=> var.
-    eapply (var_find (fun var => forall val ctxt, match bind ctxt var val with | Some ctxt' => context_srel (Complement ident (var_freevars var)) ctxt ctxt' | None => True end)
-        (fun varL => forall valL ctxt, match bind_list ctxt varL valL with
-            | Some ctxt' => context_srel (Complement ident (varl_freevars varL)) ctxt ctxt'
-            | None => True end) _ _ _ _ _ _ _ var).
-    Unshelve.
-    all: clear var; simpl.
-    {
-        move=> l HRec [| | valL] ctxt; simpl; trivial.
-        exact (HRec _ _).
-    }
-    {
-        move=> i val ctxt x HIn; simpl.
-        case_eq (String.eqb x i); simpl; trivial.
-        rewrite String.eqb_eq; move=> HEq; destruct HEq.
-        destruct HIn; constructor.
-    }
-    {
-        move=> []; simpl; trivial.
-        move=> i HRec ae val ctxt.
-        destruct (eval_arith_expr ctxt ae) as [n|]; simpl; trivial.
-        destruct (find_val ctxt i) as [[| |l]|]; simpl; trivial.
-        destruct (replace_id n l val) as [v'|]; simpl; trivial.
-        move=> x HIn; apply HRec.
-        unfold Complement; unfold In; move=> HIn'.
-        destruct HIn.
-        constructor; assumption.
-    }
-    {
-        trivial.
-    }
-    {
-        trivial.
-    }
-    {
-        move=> []; simpl; trivial.
-        reflexivity.
-    }
-    {
-        move=> varHD HRec varTL HRecL [|valHD valTL] ctxt; simpl; trivial.
-        specialize HRec with valHD ctxt.
-        destruct (bind ctxt varHD valHD) as [ctxt'|]; trivial.
-        specialize HRecL with valTL ctxt'.
-        destruct (bind_list ctxt' varTL valTL) as [ctxt'2|]; trivial.
-        transitivity ctxt'.
-        + move=> x HIn; apply HRec.
-            unfold Complement; unfold In; move=> HIn'; destruct HIn.
-            constructor; assumption.
-        + move=> x HIn; apply HRecL.
-            unfold Complement; unfold In; move=> HIn'; destruct HIn.
-            constructor; assumption.
-    }
-Qed.
-
 (* Properties about changing context *)
-
-Lemma loop_rec_eta_Some:
-    forall i1 i2 i ctxt,
-        opt_rel (context_srel (Complement ident (Singleton ident i))) (loop_rec ctxt [eta Some] i i1 i2) (Some ctxt).
-Proof.
-    move=> i1 i2; induction i2 as [|i2 HRec]; simpl.
-    by reflexivity.
-    case (match i1 with 0 => false | m'.+1 => PeanoNat.Nat.leb i2 m' end).
-    by reflexivity.
-    move=> i ctxt; specialize HRec with i ctxt.
-    destruct (loop_rec ctxt [eta Some] i i1 i2); simpl in *; trivial.
-    move=> x HIn; simpl.
-    case_eq (String.eqb x i); trivial.
-    + rewrite String.eqb_eq; move=> HEq; destruct HEq.
-        destruct HIn; constructor.
-    + move=> Snebq; apply HRec; assumption.
-Qed.
-
-Theorem expr_rel_IMP_deq_rel (arch : architecture):
-    forall e1 e2 vl b, @expr_rel arch e1 e2 -> @deq_rel arch (Eqn vl e1 b) (Eqn vl e2 b).
-Proof.
-    move=> e1 e2 vl b expr_eq.
-    unfold deq_rel; simpl.
-    unfold expr_rel in expr_eq; simpl in expr_eq.
-    intros; rewrite expr_eq.
-    apply reflexivity.
-Qed.
 
 Theorem find_val_imp_find_const:
     forall x ctxt1 ctxt2,
@@ -372,6 +283,375 @@ Proof.
     }
 Qed.
 
+Lemma context_s_rel_bind_aux_compl:
+    forall var acc val ctxt type_ctxt,
+        match bind_aux ctxt type_ctxt var acc val with
+            | Some (ctxt', l) => context_srel (Complement ident (var_freevars var)) ctxt ctxt'
+            | None => True
+        end.
+Proof.
+    move=> var; induction var as [v|v HRec ae|v HRec ae1 ae2|v HRec aeL]; simpl.
+    all: move=> acc val ctxt type_ctxt.
+    {
+        destruct (find_val type_ctxt v) as [typ|]; trivial.
+        destruct (convert_type typ nil) as [[dir form]|]; trivial.
+        pose (iL := match find_val ctxt v with | Some c => match c with | CoIL i => i::nil | CoIR _ iL _ => iL end | None => zeros (prod_list form) end).
+        fold iL.
+        destruct (update form iL acc val dir) as [[val' e']|]; trivial; clear iL.
+        move=> elt HIn; simpl.
+        case_eq (String.eqb elt v); trivial.
+        rewrite String.eqb_eq; move=> HEq; destruct HEq.
+        destruct HIn; constructor.
+    }
+    {
+        destruct (eval_arith_expr ctxt ae) as [i|]; trivial.
+        specialize HRec with (AInd i acc) val ctxt type_ctxt.
+        destruct (bind_aux ctxt type_ctxt v (AInd i acc) val) as [[ctxt' _]|]; trivial.
+        move=> elt HIn; apply HRec.
+        unfold In, Complement; move=> HIn'; destruct HIn.
+        constructor; assumption.
+    }
+    {
+        destruct (eval_arith_expr ctxt ae1) as [i1|]; trivial.
+        destruct (eval_arith_expr ctxt ae2) as [i2|]; trivial.
+        specialize HRec with (ARange i1 i2 acc) val ctxt type_ctxt.
+        destruct (bind_aux ctxt type_ctxt v (ARange i1 i2 acc) val) as [[ctxt' _]|]; trivial.
+        move=> elt HIn; apply HRec.
+        unfold In, Complement; move=> HIn'; destruct HIn.
+        constructor; assumption.
+    }
+    {
+        pose (f := fun ae l => l' <- l; x' <- eval_arith_expr ctxt ae; Some (x'::l')).
+        fold f.
+        destruct (fold_right f (Some nil) aeL) as [iL|]; trivial; clear f.
+        specialize HRec with (ASlice iL acc) val ctxt type_ctxt.
+        destruct (bind_aux ctxt type_ctxt v (ASlice iL acc) val) as [[ctxt' val']|]; trivial.
+        move=> elt HIn; apply HRec.
+        unfold In, Complement; move=> HIn'; destruct HIn.
+        constructor; assumption.
+    }
+Qed.
+
+Ltac impl_tac :=
+    lazymatch goal with
+    | |- (?A -> ?B) -> ?C =>
+        let H := fresh "H" in
+        let H2 := fresh "H" in
+        let H3 := fresh "H" in
+        assert A as H; [> idtac | (move=> H2; pose (H3 := H2 H); move: H3; clear H2 H)]
+    end.
+
+Theorem fold_right_equal {A B : Type} :
+    forall f1 f2 : A -> B -> B,
+        (forall a1 a2, f1 a1 a2 = f2 a1 a2) -> 
+        forall (l : list A), forall init : B, fold_right f1 init l = fold_right f2 init l.
+Proof.
+    move=> f1 f2 HEq l; induction l as [|h l HRec]; simpl; trivial.
+    move=> init; rewrite HEq; rewrite HRec; trivial.
+Qed.
+
+Lemma context_s_rel_bind_aux:
+    forall var acc type_ctxt ctxt1 ctxt2 val s,
+    context_srel (Union ident (var_freevars var) s) ctxt1 ctxt2 ->
+        opt_rel (fun p1 p2 => context_srel (Union ident (var_freevars var) s) p1.1 p2.1 /\ p1.2 = p2.2) (bind_aux ctxt1 type_ctxt var acc val) (bind_aux ctxt2 type_ctxt var acc val).
+Proof.
+    move=> var; induction var as [v|v HRec ae|v HRec ae1 ae2|v HRec aeL]; simpl.
+    all: move=> acc type_ctxt ctxt1 ctxt2 val s HRel.
+    {
+        destruct (find_val type_ctxt v) as [typ|]; simpl; trivial.
+        destruct (convert_type typ nil) as [[dir form]|]; simpl; trivial.
+        rewrite (HRel v).
+        2: by do 2 constructor.
+        pose (iL := match find_val ctxt2 v with | Some c => match c with | CoIL i => i::nil | CoIR _ iL _ => iL end | None => zeros (prod_list form) end).
+        fold iL.
+        destruct (update form iL acc val dir) as [[val' e']|]; simpl; trivial; clear iL.
+        split; trivial.
+        move=> elt HIn; simpl.
+        case_eq (String.eqb elt v); trivial.
+        move=> HEq; apply HRel; assumption.
+    }
+    {
+        rewrite (eval_aexpr_change_ctxt _ ctxt1 ctxt2).
+        2: move=> elt HIn; apply find_val_imp_find_const; apply HRel; do 2 constructor; assumption.
+        destruct (eval_arith_expr ctxt2 ae) as [i|]; simpl; trivial.
+        specialize HRec with (AInd i acc) type_ctxt ctxt1 ctxt2 val (Union ident (aexpr_freevars ae) s).
+        move: HRec.
+        impl_tac.
+        by rewrite <- context_srel_Union_switch; assumption.
+        destruct (bind_aux ctxt1 type_ctxt v (AInd i acc) val) as [[ctxt1' l1]|]; trivial.
+        destruct (bind_aux ctxt2 type_ctxt v (AInd i acc) val) as [[ctxt2' l2]|]; trivial.
+        simpl; move=> [HRel' ->]; split; trivial.
+        rewrite context_srel_Union_switch; assumption.
+    }
+    {
+        rewrite (eval_aexpr_change_ctxt _ ctxt1 ctxt2).
+        2: move=> elt HIn; apply find_val_imp_find_const; apply HRel; do 3 constructor; assumption.
+        rewrite (eval_aexpr_change_ctxt _ ctxt1 ctxt2).
+        2: move=> elt HIn; apply find_val_imp_find_const; apply HRel; do 3 constructor; assumption.
+        destruct (eval_arith_expr ctxt2 ae1) as [i1|]; simpl; trivial.
+        destruct (eval_arith_expr ctxt2 ae2) as [i2|]; simpl; trivial.
+        specialize HRec with (ARange i1 i2 acc) type_ctxt ctxt1 ctxt2 val (Union ident s (Union ident (aexpr_freevars ae1) (aexpr_freevars ae2))).
+        move: HRec; impl_tac.
+        by rewrite context_srel_Union2_comm; rewrite <- context_srel_Union_switch; assumption.
+        destruct (bind_aux ctxt1 type_ctxt v (ARange i1 i2 acc) val) as [[ctxt1' l1]|]; trivial.
+        destruct (bind_aux ctxt2 type_ctxt v (ARange i1 i2 acc) val) as [[ctxt2' l2]|]; trivial.
+        simpl; move=> [HRel' ->]; split; trivial.
+        rewrite context_srel_Union_switch; rewrite context_srel_Union2_comm; assumption.
+    }
+    {
+        pose (f1 := fun ae l => l' <- l; x' <- eval_arith_expr ctxt1 ae; Some (x'::l')).
+        pose (f2 := fun ae l => l' <- l; x' <- eval_arith_expr ctxt2 ae; Some (x'::l')).
+        fold f1; fold f2.
+        assert (fold_right f1 (Some nil) aeL = fold_right f2 (Some nil) aeL) as HEq.
+        {
+            unfold f1, f2; clear HRec f1 f2 acc type_ctxt val.
+            induction aeL as [|hd tl HRec]; simpl; trivial.
+            rewrite (eval_aexpr_change_ctxt hd ctxt1 ctxt2).
+            1: rewrite HRec; clear HRec.
+            + reflexivity.
+            + move=> elt HIn; apply HRel; simpl. destruct HIn as [elt' []|elt' HIn'].
+                - do 2 constructor; assumption.
+                - do 3 constructor; assumption.
+                - constructor; assumption.
+            + move=> elt HIn; apply find_val_imp_find_const; apply HRel; simpl.
+                do 3 constructor; assumption.
+        }
+        rewrite HEq; clear HEq.
+        destruct (fold_right f2 (Some nil) aeL) as [iL|]; simpl; trivial.
+        clear f1 f2.
+        specialize HRec with (ASlice iL acc) type_ctxt ctxt1 ctxt2 val (Union ident (aexprl_freevars aeL) s).
+        move: HRec; impl_tac.
+        by rewrite <-context_srel_Union_switch; assumption.
+        destruct (bind_aux ctxt1 type_ctxt v (ASlice iL acc) val) as [[ctxt1' l1]|]; trivial.
+        destruct (bind_aux ctxt2 type_ctxt v (ASlice iL acc) val) as [[ctxt2' l2]|]; trivial.
+        simpl; move=> [HRel' ->]; split; trivial.
+        rewrite context_srel_Union_switch; assumption.
+    }
+Qed.
+
+Lemma context_s_rel_bind_aux_list_compl:
+    forall varL val ctxt type_ctxt,
+        match bind_aux_list ctxt type_ctxt varL val with
+            | Some (ctxt', l) => context_srel (Complement ident (varl_freevars varL)) ctxt ctxt'
+            | None => True
+        end.
+Proof.
+    move=> varL; induction varL as [|var varL HRec]; simpl.
+    {
+        move=> [].
+        + reflexivity.
+        + by trivial.
+    }
+    {
+        move=> val ctxt type_ctxt.
+        pose (p := context_s_rel_bind_aux_compl var AAll val ctxt type_ctxt); move:p.
+        case (bind_aux ctxt type_ctxt var AAll val); trivial.
+        move=> [ctxt' val'] HRel.
+        specialize HRec with val' ctxt' type_ctxt.
+        destruct (bind_aux_list ctxt' type_ctxt varL val') as [[]|]; trivial.
+        transitivity ctxt'; move=> elt HIn.
+        + apply HRel; unfold Complement, In; move=> HIn'; destruct HIn.
+            constructor 1; unfold In; assumption.
+        + apply HRec; unfold Complement, In; move=> HIn'; destruct HIn.
+            constructor 2; unfold In; assumption.
+    }
+Qed.
+
+Lemma dec_in_aexpr_freevars:
+    forall ae elt, {In ident (aexpr_freevars ae) elt} + {not (In ident (aexpr_freevars ae) elt)}.
+Proof.
+    move=> ae elt; induction ae as [|i | op ae1 HRec1 ae2 HRec2]; simpl.
+    {
+        right; move=> HIn; destruct HIn.
+    }
+    {
+        case_eq (String.eqb i elt); move=> HEq.
+        + left; rewrite String.eqb_eq in HEq; destruct HEq; by constructor.
+        + right; move=> HEq'; destruct HEq'; rewrite String.eqb_refl in HEq; auto.
+    }
+    {
+        destruct HRec1.
+        + left; constructor; assumption.
+        + destruct HRec2.
+            - left; constructor; assumption.
+            - right; move=> HIn; destruct HIn; auto.
+    }
+Qed.
+
+Lemma dec_in_aexprl_freevars:
+    forall aeL elt, {In ident (aexprl_freevars aeL) elt} + {not (In ident (aexprl_freevars aeL) elt)}.
+Proof.
+    move=> aeL elt; induction aeL as [|hd tl HRec]; simpl.
+    {
+        right; move=> HIn; destruct HIn.
+    }
+    {
+        destruct HRec.
+        + left; constructor; assumption.
+        + destruct (dec_in_aexpr_freevars hd elt).
+            - left; constructor; assumption.
+            - right; move=> HIn; destruct HIn; auto.
+    }
+Qed.
+
+Lemma dec_in_var_freevars:
+    forall var elt, {In ident (var_freevars var) elt} + {not (In ident (var_freevars var) elt)}.
+Proof.
+    move=> var elt; induction var as [i|v HRec ae|v HRec ae1 ae2|v HRec ael]; simpl.
+    {
+        case_eq (String.eqb i elt); move=> HEq.
+        + left; rewrite String.eqb_eq in HEq; destruct HEq; by constructor.
+        + right; move=> HEq'; destruct HEq'; rewrite String.eqb_refl in HEq; auto.
+    }
+    {
+        destruct (dec_in_aexpr_freevars ae elt).
+        by left; constructor; assumption.
+        destruct HRec.
+        by left; constructor; assumption.
+        right; move=> HIn; destruct HIn; auto.
+    }
+    {
+        destruct HRec.
+        by left; constructor; assumption.
+        destruct (dec_in_aexpr_freevars ae1 elt).
+        by left; do 2 constructor; assumption.
+        destruct (dec_in_aexpr_freevars ae2 elt).
+        by left; do 2 constructor; assumption.
+        right; move=> HIn; destruct HIn as [|elt' []]; auto.
+    }
+    {
+        destruct HRec.
+        by left; constructor; assumption.
+        destruct (dec_in_aexprl_freevars ael elt).
+        by left; constructor; assumption.
+        right; move=> HIn; destruct HIn; auto.
+    }
+Qed.
+
+Lemma dec_in_varl_freevars:
+    forall varL elt, {In ident (varl_freevars varL) elt} + {not (In ident (varl_freevars varL) elt)}.
+Proof.
+    move=> varL elt; induction varL as [|hd tl HRec]; simpl.
+    {
+        right; move=> HIn; destruct HIn.
+    }
+    {
+        destruct HRec.
+        + left; constructor; assumption.
+        + destruct (dec_in_var_freevars hd elt).
+            - left; constructor; assumption.
+            - right; move=> HIn; destruct HIn; auto.
+    }
+Qed.
+
+Lemma context_s_rel_bind_aux_list:
+    forall varL type_ctxt ctxt1 ctxt2 val s,
+    context_srel (Union ident (varl_freevars varL) s) ctxt1 ctxt2 ->
+        opt_rel (fun p1 p2 => context_srel (Union ident (varl_freevars varL) s) p1.1 p2.1 /\ p1.2 = p2.2) (bind_aux_list ctxt1 type_ctxt varL val) (bind_aux_list ctxt2 type_ctxt varL val).
+Proof.
+    move=> varL; induction varL as [|var varL HRec]; simpl.
+    {
+        move=> _ ctxt1 ctxt2 []; simpl; auto.
+    }
+    {
+        move=> type_ctxt ctxt1 ctxt2 val s HRel.
+        pose (p := context_s_rel_bind_aux_compl var AAll val ctxt1 type_ctxt); move:p.
+        pose (p := context_s_rel_bind_aux_compl var AAll val ctxt2 type_ctxt); move:p.
+        pose (p := context_s_rel_bind_aux var AAll type_ctxt ctxt1 ctxt2 val s); move:p.
+        impl_tac.
+        {
+            move=> elt HIn; apply HRel; destruct HIn.
+            + do 2 constructor; assumption.
+            + constructor; assumption.
+        }
+        case (bind_aux ctxt1 type_ctxt var AAll val); simpl.
+        2: move=> ->; reflexivity.
+        case (bind_aux ctxt2 type_ctxt var AAll val); simpl.
+        2: move=> p [].
+        move=> [ctxt' val'] [ctxt'2 val'2]; simpl.
+        move=> [HRel' ->] HRel2' HRel1'2; clear val'2 val.
+        specialize HRec with type_ctxt ctxt'2 ctxt' val' (Union ident (var_freevars var) s); move: HRec.
+        impl_tac.
+        {
+            move=> elt HIn.
+            destruct HIn as [elt HIn|elt' []].
+            {
+                destruct (dec_in_var_freevars var elt).
+                + apply HRel'; constructor; assumption.
+                + rewrite <- HRel1'2.
+                    - rewrite HRel.
+                        * apply HRel2'; unfold In, Complement; assumption.
+                        * do 2 constructor; assumption.
+                    - unfold In, Complement; assumption.
+            }
+            all: apply HRel'; constructor; assumption.
+        }
+        destruct (bind_aux_list ctxt'2 type_ctxt varL val') as [[]|]; trivial.
+        destruct (bind_aux_list ctxt' type_ctxt varL val') as [[]|]; trivial; simpl.
+        rewrite <- context_srel_Union_switch; rewrite context_srel_Union1_comm; auto.
+    }
+Qed.
+
+Lemma context_srel_bind_compl:
+    forall varL val ctxt type_ctxt,
+        match bind ctxt type_ctxt varL val with
+        | Some ctxt' => context_srel (Complement ident (varl_freevars varL)) ctxt ctxt'
+        | None => True
+        end.
+Proof.
+    unfold bind.
+    move=> varL val ctxt type_ctxt.
+    pose (p := context_s_rel_bind_aux_list_compl varL val ctxt type_ctxt); move:p.
+    case (bind_aux_list ctxt type_ctxt varL val); trivial.
+    move=> []; simpl; trivial.
+    move=> ctxt' []; simpl; trivial.
+Qed.
+
+Lemma context_srel_bind:
+    forall varL type_ctxt ctxt1 ctxt2 val s,
+    context_srel (Union ident (varl_freevars varL) s) ctxt1 ctxt2 ->
+        opt_rel (context_srel (Union ident (varl_freevars varL) s)) (bind ctxt1 type_ctxt varL val) (bind ctxt2 type_ctxt varL val).
+Proof.
+    unfold bind.
+    move=> varL type_ctxt ctxt1 ctxt2 val s HRel.
+    pose (p := context_s_rel_bind_aux_list varL type_ctxt ctxt1 ctxt2 val s HRel); move:p.
+    destruct (bind_aux_list ctxt1 type_ctxt varL val) as [[ctxt1' l1]|]; simpl.
+    2: move=> ->; reflexivity.
+    destruct (bind_aux_list ctxt2 type_ctxt varL val) as [[ctxt2' l2]|]; simpl.
+    2: move=> [].
+    move=> [HRel' ->].
+    destruct l2; simpl; auto.
+Qed.
+
+(* Properties about changing context *)
+
+Lemma loop_rec_eta_Some:
+    forall i1 i2 i ctxt,
+        opt_rel (context_srel (Complement ident (Singleton ident i))) (loop_rec ctxt [eta Some] i i1 i2) (Some ctxt).
+Proof.
+    move=> i1 i2; induction i2 as [|i2 HRec]; simpl.
+    by reflexivity.
+    case (match i1 with 0 => false | m'.+1 => PeanoNat.Nat.leb i2 m' end).
+    by reflexivity.
+    move=> i ctxt; specialize HRec with i ctxt.
+    destruct (loop_rec ctxt [eta Some] i i1 i2); simpl in *; trivial.
+    move=> x HIn; simpl.
+    case_eq (String.eqb x i); trivial.
+    + rewrite String.eqb_eq; move=> HEq; destruct HEq.
+        destruct HIn; constructor.
+    + move=> Snebq; apply HRec; assumption.
+Qed.
+
+Theorem expr_rel_IMP_deq_rel (arch : architecture):
+    forall e1 e2 vl b, @expr_rel arch e1 e2 -> @deq_rel arch (Eqn vl e1 b) (Eqn vl e2 b).
+Proof.
+    move=> e1 e2 vl b expr_eq.
+    unfold deq_rel; simpl.
+    unfold expr_rel in expr_eq; simpl in expr_eq.
+    intros; rewrite expr_eq.
+    apply reflexivity.
+Qed.
+
 Ltac eq_match :=
     lazymatch goal with
     | |- match ?A with Some _ => _ | None => _ end = match ?B with Some _ => _ | None => _  end =>
@@ -379,54 +659,69 @@ Ltac eq_match :=
         assert (A = B) as H; [> idtac | rewrite H; reflexivity]
     end.
 
-Theorem eval_var_change_ctxt:
-    (forall v ctxt1 ctxt2,
-        context_srel (var_freevars v) ctxt1 ctxt2 ->
-        eval_var ctxt1 v = eval_var ctxt2 v).
+Ltac small_eq_match :=
+    lazymatch goal with
+    | |- match ?A with Some _ => _ | None => _ end = match ?B with Some _ => _ | None => _  end =>
+        let H := fresh "H" in
+        assert (A = B) as H; [> idtac | rewrite H; destruct B]
+    end.
+
+Theorem fold_left_equal {A B : Type} :
+    forall f1 f2 : A -> B -> A,
+        (forall a1 a2, f1 a1 a2 = f2 a1 a2) -> 
+        forall (l : list B), forall init : A, fold_left f1 l init = fold_left f2 l init.
 Proof.
-    apply (var_find
-        (fun v => forall ctxt1 ctxt2,
-            context_srel (var_freevars v) ctxt1 ctxt2 ->
-            eval_var ctxt1 v = eval_var ctxt2 v)
-        (fun v => forall ctxt1 ctxt2,
-            context_srel (varl_freevars v) ctxt1 ctxt2 ->
-            eval_vars ctxt1 v = eval_vars ctxt2 v)); simpl.
-    + move=> l HRec ctxt1 ctxt2 HImpl; rewrite (HRec ctxt1 ctxt2).
-        - reflexivity.
-        - move=> x HIn; apply HImpl; assumption.
-    + move=> i ctxt1 ctxt2 ->; trivial.
-        - constructor.
-    + move=> v HRec ae ctxt1 ctxt2 HContent; rewrite (eval_aexpr_change_ctxt _ ctxt1 ctxt2).
-        - rewrite (HRec ctxt1 ctxt2).
-            * reflexivity.
-            * move=> x HIn; apply HContent; constructor; assumption.
-        - move=> x HIn; apply find_val_imp_find_const; apply HContent; constructor; assumption.
-    + move=> v HRec ae1 ae2 ctxt1 ctxt2 HContent; rewrite (eval_aexpr_change_ctxt _ ctxt1 ctxt2).
-        - rewrite (eval_aexpr_change_ctxt _ ctxt1 ctxt2).
-            * rewrite (HRec ctxt1 ctxt2); trivial.
-                by move=> x HIn; apply HContent; constructor; assumption.
-            * move=> x HIn; apply find_val_imp_find_const; apply HContent; do 2 constructor; assumption.
-        - move=> x HIn; apply find_val_imp_find_const; apply HContent; do 2 constructor; assumption.
-    + move=> v HRec ael ctxt1 ctxt2 HContent.
-        rewrite (HRec ctxt1 ctxt2).
-        2: by move=> x HIn; apply HContent; constructor; assumption.
-        eq_match.
-        clear HRec.
-        move: HContent.
-        induction ael as [|a tl HRec]; simpl; trivial.
-        move=> HContent.
+    move=> f1 f2 HEq l; induction l as [|h l HRec]; simpl; trivial.
+    move=> init; rewrite HEq; rewrite HRec; trivial.
+Qed.
+
+Theorem eval_var_change_ctxt:
+    forall v ctxt1 ctxt2 acc,
+        context_srel (var_freevars v) ctxt1 ctxt2 ->
+        eval_var ctxt1 v acc = eval_var ctxt2 v acc.
+Proof.
+    move=> v ctxt1 ctxt2; induction v as [|v HRec ind| v HRec ind1 ind2| v HRec indL]; simpl; move=> acc HRel.
+    {
+        rewrite HRel.
+        2: by constructor.
+        destruct (find_val ctxt2 i) as [|]; trivial.
+    }
+    {
         rewrite (eval_aexpr_change_ctxt _ ctxt1 ctxt2).
-        2: by move=> x HIn; apply find_val_imp_find_const; apply HContent; constructor; constructor; assumption.
-        eq_match.
-        apply HRec.
-        move=> x HIn; apply HContent; inversion HIn.
-        - constructor; assumption.
-        - do 2 constructor; assumption.
-    + reflexivity.
-    + move=> v HRec vL HRecL ctxt1 ctxt2 HContent; rewrite (HRec ctxt1 ctxt2).
-        - rewrite (HRecL ctxt1 ctxt2); trivial.
-            * move=> x HIn; apply HContent; constructor; assumption.
-        - move=> x HIn; apply HContent; constructor; assumption.
+        2: move=> x HIn; apply find_val_imp_find_const; apply HRel; constructor; assumption.
+        case (eval_arith_expr ctxt2 ind); trivial.
+        move=> n; apply HRec.
+        move=> elt HIn; apply HRel; constructor; assumption.
+    }
+    {
+        rewrite (eval_aexpr_change_ctxt _ ctxt1 ctxt2).
+        2: move=> x HIn; apply find_val_imp_find_const; apply HRel; do 2 constructor; assumption.
+        rewrite (eval_aexpr_change_ctxt _ ctxt1 ctxt2).
+        2: move=> x HIn; apply find_val_imp_find_const; apply HRel; do 2 constructor; assumption.
+        case (eval_arith_expr ctxt2 ind1); trivial.
+        case (eval_arith_expr ctxt2 ind2); trivial.
+        move=> n1 n2; rewrite HRec; trivial.
+        move=> elt HIn; apply HRel.
+        constructor; assumption.
+    }
+    {
+        small_eq_match; trivial.
+        2: apply HRec; move=> elt HIn; apply HRel; constructor; assumption.
+        clear HRec.
+        induction indL as [|hd tl HRec]; simpl; trivial.
+        small_eq_match; trivial.
+        {
+            apply HRec.
+            move=> elt HIn; apply HRel; simpl; destruct HIn.
+            + constructor; assumption.
+            + do 2 constructor; assumption.
+        }
+        {
+            eq_match; apply eval_aexpr_change_ctxt.
+            move=> elt HIn; apply find_val_imp_find_const.
+            apply HRel; do 2 constructor; assumption.
+        }
+    }
 Qed.
 
 Theorem eval_expr_change_ctxt (arch : architecture) (prog : prog_ctxt):
@@ -479,89 +774,6 @@ Proof.
         move => x HIn; apply HContent; constructor; assumption.
 Qed.
 
-Lemma context_srel_bind:
-    forall var ctxt1 ctxt2 val s,
-        context_srel (Union ident (var_freevars var) s) ctxt1 ctxt2 ->
-            opt_rel (context_srel (Union ident (var_freevars var) s)) (bind ctxt1 var val) (bind ctxt2 var val).
-Proof.
-    move=> var.
-    eapply (var_find (fun var => forall (ctxt1 ctxt2 : context) (val : Value) (s : Ensemble ident),
-        context_srel (Union ident (var_freevars var) s) ctxt1 ctxt2 -> opt_rel (context_srel (Union ident (var_freevars var) s))
-        (bind ctxt1 var val) (bind ctxt2 var val)) (fun varl => forall (ctxt1 ctxt2 : context) (valL : list_Value) (s : Ensemble ident),
-            context_srel (Union ident (varl_freevars varl) s) ctxt1 ctxt2 -> opt_rel (context_srel (Union ident (varl_freevars varl) s)) (bind_list ctxt1 varl valL) (bind_list ctxt2 varl valL)) _ _ _ _ _ _ _ var).
-    Unshelve.
-    all: simpl.
-    {
-        move=> l HRec ctxt1 ctxt2 []; simpl; trivial.
-        move=> vL s HRel; apply HRec; auto.
-    }
-    {
-        move=> i ctxt1 ctxt2 val s HRel x HIn; simpl.
-        case (String.eqb x i); simpl; trivial.
-        apply HRel; assumption.
-    }
-    {
-        move=> []; simpl; trivial.
-        move=> i HRec ae ctxt1 ctxt2 val s HRel.
-        rewrite (eval_aexpr_change_ctxt _ ctxt1 ctxt2).
-        2: by move=> x HIn; apply find_val_imp_find_const; apply HRel; do 2 constructor; assumption.
-        rewrite (HRel i).
-        2: by do 3 constructor; assumption.
-        case (eval_arith_expr ctxt2 ae); simpl; trivial; move=> n.
-        case (find_val ctxt2 i); simpl; trivial.
-        move=> []; simpl; trivial.
-        move=> l; case (replace_id n l val); simpl; trivial.
-        move=> l0 x HIn; simpl.
-        case (String.eqb x i); trivial.
-        apply HRel; trivial.
-    }
-    {
-        reflexivity.
-    }
-    {
-        reflexivity.
-    }
-    {
-        move=> ctxt1 ctxt2 []; simpl; trivial.
-    }
-    {
-        move=> v HRec l HRecL ctxt1 ctxt2 []; simpl; trivial.
-        move=> valHD valTL s HRel.
-        assert (context_srel (Union ident (var_freevars v) (Union ident s (varl_freevars l))) ctxt1 ctxt2) as HRel'.
-        { 
-            move=> x HIn; apply HRel; destruct HIn as [|x HIn].
-                + do 2 constructor; assumption.
-                + destruct HIn.
-                    - constructor; assumption.
-                    - do 2 constructor; assumption.
-        }
-        pose (p := HRec _ _ valHD _ HRel'); move:p.
-        case (bind ctxt1 v valHD); simpl.
-        2: by move=> ->; simpl; reflexivity.
-        case (bind ctxt2 v valHD); simpl.
-        2: by move=> _ [].
-        clear HRec HRel HRel' valHD var ctxt1 ctxt2.
-        move=> ctxt1 ctxt2 HRel.
-        rewrite (opt_rel_context_srel_change_set _ _ (context_srel_Union1_comm _ _ _) _ _).
-        rewrite (opt_rel_context_srel_change_set _ _ (context_srel_Union_switch _ _ _) _ _).
-        apply HRecL.
-        rewrite <- context_srel_Union_switch.
-        rewrite context_srel_Union1_comm.
-        rewrite context_srel_Union_switch.
-        rewrite context_srel_Union2_comm.
-        assumption.
-    }
-Qed.
-
-Theorem fold_left_equal {A B : Type} :
-    forall f1 f2 : A -> B -> A,
-        (forall a1 a2, f1 a1 a2 = f2 a1 a2) -> 
-        forall (l : list B), forall init : A, fold_left f1 l init = fold_left f2 l init.
-Proof.
-    move=> f1 f2 HEq l; induction l as [|h l HRec]; simpl; trivial.
-    move=> init; rewrite HEq; rewrite HRec; trivial.
-Qed.
-
 Lemma loop_rec_equiv:
     forall f1 f2,
         (forall a, f1 a = f2 a) ->
@@ -577,7 +789,7 @@ Qed.
 
 Inductive deqL :=
     | DLnil
-    | DLEqn : var -> expr -> bool -> deqL -> deqL
+    | DLEqn : list var -> expr -> bool -> deqL -> deqL
     | DLLoop : ident -> arith_expr -> arith_expr -> deqL -> list stmt_opt -> deqL -> deqL.
 
 Fixpoint deqL_of_list_deq (d : list_deq) : deqL :=
@@ -611,24 +823,24 @@ Proof.
 Qed.
 
 Lemma eval_deqL_change_ctxt arch prog:
-    forall eqns ctxt1 ctxt2 s,
+    forall eqns type_ctxt ctxt1 ctxt2 s,
         (forall elt, In ident (deqs_vars (list_deq_of_deqL eqns)) elt -> In ident s elt)
         -> context_srel s ctxt1 ctxt2
         -> opt_rel (context_srel s)
-            (eval_deq_list arch prog ctxt1 (list_deq_of_deqL eqns))
-            (eval_deq_list arch prog ctxt2 (list_deq_of_deqL eqns)).
+            (eval_deq_list arch prog type_ctxt ctxt1 (list_deq_of_deqL eqns))
+            (eval_deq_list arch prog type_ctxt ctxt2 (list_deq_of_deqL eqns)).
 Proof.
     move=> eqns; induction eqns as [|v e b tl HRec|i a1 a2 body HRecBody opt tl HRecTL]; simpl; auto.
     {
-        move=> ctxt1 ctxt2 s HSubset HRel.
+        move=> type_ctxt ctxt1 ctxt2 s HSubset HRel.
         rewrite (eval_expr_change_ctxt _ _ _ ctxt1 ctxt2).
         2: by move=> x HIn; apply HRel; apply HSubset; do 2 constructor; assumption.
         destruct (eval_expr arch prog ctxt2 e) as [val|].
         2: reflexivity.
-        assert (context_srel (Union ident (var_freevars v) s) ctxt1 ctxt2) as HRel'
+        assert (context_srel (Union ident (varl_freevars v) s) ctxt1 ctxt2) as HRel'
         by (move=> x [x' HIn|x' HIn]; apply HRel; trivial; apply HSubset; do 2 constructor; assumption).
-        pose (p := context_srel_bind _ _ _ val _ HRel'); move:p; clear HRel'.
-        destruct (bind ctxt1 v val) as [ctxt1'|]; destruct (bind ctxt2 v val) as [ctxt2'|]; simpl.
+        pose (p := context_srel_bind _ type_ctxt _ _ val _ HRel'); move:p; clear HRel'.
+        destruct (bind ctxt1 type_ctxt v val) as [ctxt1'|]; destruct (bind ctxt2 type_ctxt v val) as [ctxt2'|]; simpl.
         2: move=> [].
         2: discriminate.
         2: reflexivity.
@@ -637,7 +849,7 @@ Proof.
         + move=> x HIn; apply HRel'; constructor; assumption.
     }
     {
-        move=> ctxt1 ctxt2 s HSubset HRel.
+        move=> type_ctxt ctxt1 ctxt2 s HSubset HRel.
         rewrite (eval_aexpr_change_ctxt a1 ctxt1 ctxt2).
         2: move=> x HIn; apply find_val_imp_find_const; apply HRel; apply HSubset; do 3 constructor; assumption.
         rewrite (eval_aexpr_change_ctxt a2 ctxt1 ctxt2).
@@ -645,8 +857,8 @@ Proof.
         destruct (eval_arith_expr ctxt2 a1) as [i1|]; simpl; trivial.
         destruct (eval_arith_expr ctxt2 a2) as [i2|]; simpl; trivial.
         assert (opt_rel (context_srel s)
-                (loop_rec ctxt1 ((eval_deq_list arch prog)^~ (list_deq_of_deqL body)) i i1 i2)
-                (loop_rec ctxt2 ((eval_deq_list arch prog)^~ (list_deq_of_deqL body)) i i1 i2))
+                (loop_rec ctxt1 ((eval_deq_list arch prog type_ctxt)^~ (list_deq_of_deqL body)) i i1 i2)
+                (loop_rec ctxt2 ((eval_deq_list arch prog type_ctxt)^~ (list_deq_of_deqL body)) i i1 i2))
             as HLoop.
         {
             assert (forall elt, In ident (deqs_vars (list_deq_of_deqL body)) elt -> In ident s elt) as HSubset'
@@ -654,18 +866,18 @@ Proof.
             clear HSubset HRecTL a1 a2 tl.
             induction i2 as [|i2 HReci]; simpl; auto.
             case (match i1 with 0 => false | m'.+1 => PeanoNat.Nat.leb i2 m' end); simpl; trivial.
-            destruct (loop_rec ctxt1 ((eval_deq_list arch prog)^~ (list_deq_of_deqL body)) i i1 i2) as [ctxt1'|].
+            destruct (loop_rec ctxt1 ((eval_deq_list arch prog type_ctxt)^~ (list_deq_of_deqL body)) i i1 i2) as [ctxt1'|].
             2: simpl in HReci; rewrite HReci; reflexivity.
-            destruct (loop_rec ctxt2 ((eval_deq_list arch prog)^~ (list_deq_of_deqL body)) i i1 i2) as [ctxt2'|].
+            destruct (loop_rec ctxt2 ((eval_deq_list arch prog type_ctxt)^~ (list_deq_of_deqL body)) i i1 i2) as [ctxt2'|].
             all: simpl in HReci.
             2: by destruct HReci.
             apply HRecBody; trivial.
             move=> x HIn; simpl.
             case (String.eqb x i); trivial; apply HReci; assumption.
         }
-        destruct (loop_rec ctxt1 ((eval_deq_list arch prog)^~ (list_deq_of_deqL body)) i i1 i2) as [ctxt1'|].
+        destruct (loop_rec ctxt1 ((eval_deq_list arch prog type_ctxt)^~ (list_deq_of_deqL body)) i i1 i2) as [ctxt1'|].
         2: simpl in HLoop; rewrite HLoop; reflexivity.
-        destruct (loop_rec ctxt2 ((eval_deq_list arch prog)^~ (list_deq_of_deqL body)) i i1 i2) as [ctxt2'|].
+        destruct (loop_rec ctxt2 ((eval_deq_list arch prog type_ctxt)^~ (list_deq_of_deqL body)) i i1 i2) as [ctxt2'|].
         all: simpl in HLoop.
         2: by destruct HLoop.
         assert (match find_val ctxt1 i with Some v => Some ((i, v) :: ctxt1') | None => Some ctxt1' end
@@ -700,8 +912,8 @@ Qed.
 
 
 Lemma eval_deq_list_unchanged_ctxt arch prog:
-    forall eqns ctxt,
-        match eval_deq_list arch prog ctxt (list_deq_of_deqL eqns) with
+    forall eqns type_ctxt ctxt,
+        match eval_deq_list arch prog type_ctxt ctxt (list_deq_of_deqL eqns) with
         | None => True
         | Some ctxt' => context_srel (Complement ident (deqs_boundvars (list_deq_of_deqL eqns))) ctxt ctxt'
         end.
@@ -709,12 +921,12 @@ Proof.
     move=> eqns; induction eqns as [|var e b tl HRecTL| i a1 a2 body HRecBody opt tl HRecTL]; simpl.
     { reflexivity. }
     {
-        move=> ctxt.
+        move=> type_ctxt ctxt.
         destruct (eval_expr arch prog ctxt e) as [val|]; simpl; trivial.
-        pose (p := context_srel_bind_compl var val ctxt); move:p.
-        destruct (bind ctxt var val) as [ctxt'|]; simpl; trivial.
-        specialize HRecTL with ctxt'.
-        destruct (eval_deq_list arch prog ctxt' (list_deq_of_deqL tl)) as [ctxt'2|]; trivial.
+        pose (p := context_srel_bind_compl var val ctxt type_ctxt); move:p.
+        destruct (bind ctxt type_ctxt var val) as [ctxt'|]; simpl; trivial.
+        specialize HRecTL with type_ctxt ctxt'.
+        destruct (eval_deq_list arch prog type_ctxt ctxt' (list_deq_of_deqL tl)) as [ctxt'2|]; trivial.
         move=> HRel; transitivity ctxt'; move=> x HIn.
         + apply HRel; unfold Complement; unfold In; move=> not_var.
             destruct HIn; constructor 1; unfold In; assumption.
@@ -722,10 +934,10 @@ Proof.
             destruct HIn; constructor 2; unfold In; assumption.
     }
     {
-        move=> ctxt.
+        move=> type_ctxt ctxt.
         destruct (eval_arith_expr ctxt a1) as [i1|]; simpl; trivial.
         destruct (eval_arith_expr ctxt a2) as [i2|]; simpl; trivial.
-        assert (match loop_rec ctxt ((eval_deq_list arch prog)^~ (list_deq_of_deqL body)) i i1 i2 with
+        assert (match loop_rec ctxt ((eval_deq_list arch prog type_ctxt)^~ (list_deq_of_deqL body)) i i1 i2 with
             | None => True
             | Some ctxt' => context_srel (Complement ident (Union ident (Singleton ident i) (deqs_boundvars (list_deq_of_deqL body)))) ctxt ctxt'
             end) as HLoop.
@@ -734,9 +946,9 @@ Proof.
             { reflexivity. }
             case (match i1 with 0 => false | m'.+1 => PeanoNat.Nat.leb i2 m' end).
             { reflexivity. }
-            destruct (loop_rec ctxt ((eval_deq_list arch prog)^~(list_deq_of_deqL body)) i i1 i2) as [ctxt'|]; trivial.
-            specialize HRecBody with ((i, VConst i2) :: ctxt').
-            destruct (eval_deq_list arch prog ((i, VConst i2)::ctxt') (list_deq_of_deqL body)) as [ctxt'2|]; trivial.
+            destruct (loop_rec ctxt ((eval_deq_list arch prog type_ctxt)^~(list_deq_of_deqL body)) i i1 i2) as [ctxt'|]; trivial.
+            specialize HRecBody with type_ctxt ((i, CoIL i2) :: ctxt').
+            destruct (eval_deq_list arch prog type_ctxt ((i, CoIL i2)::ctxt') (list_deq_of_deqL body)) as [ctxt'2|]; trivial.
             transitivity ctxt'; trivial.
             move=> elt HIn; rewrite <- HRecBody.
             + simpl.
@@ -747,11 +959,11 @@ Proof.
             + unfold Complement, In; intro; destruct HIn; constructor 2; unfold In; assumption.
         }
         clear HRecBody.
-        destruct (loop_rec ctxt ((eval_deq_list arch prog)^~(list_deq_of_deqL body)) i i1 i2) as [ctxt'|]; trivial.
-        specialize HRecTL with (match find_val ctxt i with Some v => (i,v)::ctxt' | None=> ctxt' end).
+        destruct (loop_rec ctxt ((eval_deq_list arch prog type_ctxt)^~(list_deq_of_deqL body)) i i1 i2) as [ctxt'|]; trivial.
+        specialize HRecTL with type_ctxt (match find_val ctxt i with Some v => (i,v)::ctxt' | None=> ctxt' end).
         destruct (find_val ctxt i) as [val|].
         {
-            destruct (eval_deq_list arch prog ((i, val)::ctxt') (list_deq_of_deqL tl)) as [ctxt'2|]; trivial.
+            destruct (eval_deq_list arch prog type_ctxt ((i, val)::ctxt') (list_deq_of_deqL tl)) as [ctxt'2|]; trivial.
             transitivity ctxt'; move=> x HIn.
             {
                 apply HLoop; unfold Complement; unfold In; move=> HProp.
@@ -768,7 +980,7 @@ Proof.
             + unfold Complement, In; intro; destruct HIn; constructor 2; unfold In; assumption.
         }
         {
-            destruct (eval_deq_list arch prog ctxt' (list_deq_of_deqL tl)) as [ctxt'2|]; trivial.
+            destruct (eval_deq_list arch prog type_ctxt ctxt' (list_deq_of_deqL tl)) as [ctxt'2|]; trivial.
             transitivity ctxt'; move=> x HIn.
             {
                 apply HLoop; unfold Complement; unfold In; move=> HProp.
@@ -784,19 +996,19 @@ Proof.
 Qed.
 
 Lemma loop_rec_unchanged_ctxt arch prog:
-    forall i i1 i2 body ctxt,
-        match loop_rec ctxt ((eval_deq_list arch prog)^~ (list_deq_of_deqL body)) i i1 i2 with
+    forall i i1 i2 body ctxt type_ctxt,
+        match loop_rec ctxt ((eval_deq_list arch prog type_ctxt)^~ (list_deq_of_deqL body)) i i1 i2 with
         | None => True
         | Some ctxt' => context_srel (Complement ident (Union ident (Singleton ident i) (deqs_boundvars (list_deq_of_deqL body)))) ctxt ctxt'
         end.
 Proof.
-    move=> i i1 i2 body ctxt; induction i2 as [|i2 HRec]; simpl.
+    move=> i i1 i2 body ctxt type_ctxt; induction i2 as [|i2 HRec]; simpl.
     { reflexivity. }
     case (match i1 with 0 => false | m'.+1 => PeanoNat.Nat.leb i2 m' end).
     { reflexivity. }
-    destruct (loop_rec ctxt ((eval_deq_list arch prog)^~ (list_deq_of_deqL body)) i i1 i2) as [ctxt'|]; trivial.
-    pose (p := eval_deq_list_unchanged_ctxt arch prog body ((i, VConst i2)::ctxt')); move:p.
-    destruct (eval_deq_list arch prog ((i, VConst i2)::ctxt') (list_deq_of_deqL body)) as [ctxt'2|]; trivial.
+    destruct (loop_rec ctxt ((eval_deq_list arch prog type_ctxt)^~ (list_deq_of_deqL body)) i i1 i2) as [ctxt'|]; trivial.
+    pose (p := eval_deq_list_unchanged_ctxt arch prog body type_ctxt ((i, CoIL i2)::ctxt')); move:p.
+    destruct (eval_deq_list arch prog type_ctxt ((i, CoIL i2)::ctxt') (list_deq_of_deqL body)) as [ctxt'2|]; trivial.
     move=> HBody; transitivity ctxt'; trivial.
     move=> elt HIn; rewrite <- HBody.
     + simpl.
